Code cleanup w/ identifier case standards

uvmMemoryModelScript.sml
@@ -8,7 +8,7 @@ val _ = new_theory "uvmMemoryModel";
 
 
 (* Datatypes and type abbreviations *)
-val _ = type_abbrev("input", ``:(memoryMessage # tid)``);
+val _ = type_abbrev("input", ``:(memory_message # tid)``);
 val _ = Datatype` output_message = Out value memreqid tid `;
 val _ = Datatype`ops = Rd | Wr | Fn `;
 val _ = Datatype`
@@ -20,56 +20,57 @@ val _ = Datatype`
     thread_id : tid ;
     order     : memoryorder ;
     ddeps     : memdeps
-  |>`
+  |>
+`;
 val _ = Datatype`
   graph = <|
-          nodes : node list ;
-             rf : node |-> node
-          |>`;
-
+    nodes : node list ;
+    rf    : node |-> node
+  |>
+`;
 
 (* Term definitions *)
-val isFence_def = Define`
-    isFence n = (n.operation = Fn)`;
+val is_fence_def = Define`
+    is_fence n = (n.operation = Fn)`;
 
-val isLoad_def = Define`
-    isLoad n = (n.operation = Rd)`;
+val is_load_def = Define`
+    is_load n = (n.operation = Rd)`;
 
-val isStore_def = Define`
-    isStore n = (n.operation = Wr)`;
+val is_store_def = Define`
+    is_store n = (n.operation = Wr)`;
 
-val isAcquire_def = Define`
-    isAcquire n = case n.order of
+val is_acquire_def = Define`
+    is_acquire n = case n.order of
         ACQUIRE => (n.operation = Rd) ∨ (n.operation = Fn)
       | ACQ_REL => (n.operation = Rd) ∨ (n.operation = Fn)
       | SEQ_CST => (n.operation = Rd) ∨ (n.operation = Fn)
       | CONSUME => (n.operation = Fn)
       | _       => F`;
 
-val isConsume_def = Define`
-    isConsume n = ((n.operation = Rd) ∧ (n.order <> NOT_ATOMIC) ∧ (n.order <> RELAXED)) (* or (n.order=CONSUME) *)`;
+val is_consume_def = Define`
+    is_consume n = ((n.operation = Rd) ∧ (n.order <> NOT_ATOMIC) ∧ (n.order <> RELAXED)) (* or (n.order=CONSUME) *)`;
 
-val isRelease_def = Define`
-    isRelease n = case n.order of
+val is_release_def = Define`
+    is_release n = case n.order of
         RELEASE => (n.operation = Wr) ∨ (n.operation = Fn)
       | ACQ_REL => (n.operation = Wr) ∨ (n.operation = Fn)
       | SEQ_CST => (n.operation = Wr) ∨ (n.operation = Fn)
       | _       => F`;
 
-val isSeqCst_def = Define`
-    isSeqCst n = (n.order = SEQ_CST)`;
+val is_seq_cst_def = Define`
+    is_seq_cst n = (n.order = SEQ_CST)`;
 
-val isAtomic_def = Define`
-    isAtomic n = (n.order <> NOT_ATOMIC)`;
+val is_atomic_def = Define`
+    is_atomic n = (n.order <> NOT_ATOMIC)`;
 
-val sameThread_def = Define`
-    sameThread A B = (A.thread_id = B.thread_id)`;
+val same_thread_def = Define`
+    same_thread A B = (A.thread_id = B.thread_id)`;
 
-val sameAddress_def = Define`
-    sameAddress A B = (A.address = B.address)`;
+val same_address_def = Define`
+    same_address A B = (A.address = B.address)`;
 
-val isInGraph_def = Define`
-    isInGraph g A = MEM A g.nodes`;
+val is_in_graph_def = Define`
+    is_in_graph g A = MEM A g.nodes`;
 
 
 
@@ -77,93 +78,93 @@ val isInGraph_def = Define`
 
 
 (* Undefined for missing items *)
-val orderedBefore_def = Define`
-    orderedBefore g A B = ((isInGraph g A) ∧ (isInGraph g B) ∧ (THE (INDEX_OF A g.nodes)) < (THE (INDEX_OF B g.nodes)))`;
+val ordered_before_def = Define`
+    ordered_before g A B = ((is_in_graph g A) ∧ (is_in_graph g B) ∧ (THE (INDEX_OF A g.nodes)) < (THE (INDEX_OF B g.nodes)))`;
     (*             of
                               (SOME a, SOME b) => (a < b)
                             | _ => (F)  `;*)
 
-val isReadBy_def = Define`
-    isReadBy g A B = (FLOOKUP g.rf B = SOME A)`;
+val is_read_by_def = Define`
+    is_read_by g A B = (FLOOKUP g.rf B = SOME A)`;
 
-val modifiesBefore_def = Define`
-    modifiesBefore g A B = ( (orderedBefore g A B) ∧ (sameAddress A B) ∧ (isStore A) ∧ (isStore B))`;
+val modifies_before_def = Define`
+    modifies_before g A B = ( (ordered_before g A B) ∧ (same_address A B) ∧ (is_store A) ∧ (is_store B))`;
 
-val sequencedBefore_def = Define`
-    sequencedBefore g A B = ((orderedBefore g A B) ∧ (sameThread A B)  )`;
+val sequenced_before_def = Define`
+    sequenced_before g A B = ((ordered_before g A B) ∧ (same_thread A B)  )`;
 
-val inReleaseSequenceOf_def = Define`
-    inReleaseSequenceOf g B A = ( ((B = A) ∧ (isInGraph g A)) ∨ ((modifiesBefore g A B) ∧ (isAtomic B) ∧ (sequencedBefore g A B)))`;
-val releaseSequenceOf_def = Define` (* TODO: include read-write ops *)
-    releaseSequenceOf g A = { B | (B = A) ∨ ((modifiesBefore g A B) ∧ (isAtomic B) ∧ (isStore B) ∧ ((sequencedBefore g A B) ∨ (F) )  )}   `;
+val in_release_sequence_of_def = Define`
+    in_release_sequence_of g B A = ( ((B = A) ∧ (is_in_graph g A)) ∨ ((modifies_before g A B) ∧ (is_atomic B) ∧ (sequenced_before g A B)))`;
+val release_sequence_of_def = Define` (* TODO: include read-write ops *)
+    release_sequence_of g A = { B | (B = A) ∨ ((modifies_before g A B) ∧ (is_atomic B) ∧ (is_store B) ∧ ((sequenced_before g A B) ∨ (F) )  )}   `;
 
-val carriesDependencyTo_def = Define`
-    carriesDependencyTo g A B = ((A.mid IN B.ddeps) ∧ (isInGraph g A) ∧ (isInGraph g B))`;
+val carries_dependency_to_def = Define`
+    carries_dependency_to g A B = ((A.mid IN B.ddeps) ∧ (is_in_graph g A) ∧ (is_in_graph g B))`;
 (* This should be worked out within the thread? *)
 (* val (cdep_rules, cdep_ind, cdep_cases) = Hol_reln` (* This might not be how reln is supposed to work *)
-    (∀ g B A. (A.mid IN B.ddeps) ==> (carriesDependencyTo g B A)) ∧
-    (∀ g B A. (∃ X. (sequencedBefore g A X) ∧ (sequencedBefore g X B) ∧ (isStore X) ∧ (isLoad B) ∧ (sameAddress X B) ∧ (A.mid IN X.ddeps)) ==> (carriesDependencyTo g B A)) ∧
-    (∀ g B A. (∃ X. (carriesDependencyTo g A X) ∧ (carriesDependencyTo g X B)) ==> (carriesDependencyTo g B A) )`;*)
+    (∀ g B A. (A.mid IN B.ddeps) ==> (carries_dependency_to g B A)) ∧
+    (∀ g B A. (∃ X. (sequenced_before g A X) ∧ (sequenced_before g X B) ∧ (is_store X) ∧ (is_load B) ∧ (same_address X B) ∧ (A.mid IN X.ddeps)) ==> (carries_dependency_to g B A)) ∧
+    (∀ g B A. (∃ X. (carries_dependency_to g A X) ∧ (carries_dependency_to g X B)) ==> (carries_dependency_to g B A) )`;*)
 
-val synchronizesWith_def = Define`
-    synchronizesWith g A B = (
-        (*1.*) ( (isRelease A) ∧ (isAcquire B) ∧ (sameAddress A B) ∧ (∃ X. (isReadBy g X B ) ∧ (inReleaseSequenceOf g X A)) ) ∨
-        (*2.*) ( (isRelease A) ∧ (isAcquire B) ∧ (isFence A) ∧ (isFence B) ∧ (∃ X Y. (isAtomic X) ∧ (isAtomic Y) ∧ (sameAddress X Y) ∧ (sequencedBefore g A X) ∧ (isStore X) ∧ (sequencedBefore g Y B) ∧ ( (isReadBy g X Y) ∨ (∃ Z. (isReadBy g Z Y) ∧ (inReleaseSequenceOf g Z X)))) ) ∨
-        (*3.*) ( (isRelease A) ∧ (isAcquire B) ∧ (isFence A) ∧ (∃ X. (sequencedBefore g A X) ∧ (sameAddress B X) ∧ ((isReadBy g X B) ∨ (∃ Z. (isReadBy g Z B) ∧ (inReleaseSequenceOf g Z X))) ) ) ∨
-        (*4.*) ( (isAtomic A) ∧ (isRelease A) ∧ (isAcquire B) ∧ (isFence B) ∧ (∃ X. (sameAddress A X) ∧ (sequencedBefore g X B) ∧ ((isReadBy g A X) ∨ (∃ Z. (isReadBy g Z X) ∧ (inReleaseSequenceOf g Z A))  ))  ) ∨ (* TODO *)
+val synchronizes_with_def = Define`
+    synchronizes_with g A B = (
+        (*1.*) ( (is_release A) ∧ (is_acquire B) ∧ (same_address A B) ∧ (∃ X. (is_read_by g X B ) ∧ (in_release_sequence_of g X A)) ) ∨
+        (*2.*) ( (is_release A) ∧ (is_acquire B) ∧ (is_fence A) ∧ (is_fence B) ∧ (∃ X Y. (is_atomic X) ∧ (is_atomic Y) ∧ (same_address X Y) ∧ (sequenced_before g A X) ∧ (is_store X) ∧ (sequenced_before g Y B) ∧ ( (is_read_by g X Y) ∨ (∃ Z. (is_read_by g Z Y) ∧ (in_release_sequence_of g Z X)))) ) ∨
+        (*3.*) ( (is_release A) ∧ (is_acquire B) ∧ (is_fence A) ∧ (∃ X. (sequenced_before g A X) ∧ (same_address B X) ∧ ((is_read_by g X B) ∨ (∃ Z. (is_read_by g Z B) ∧ (in_release_sequence_of g Z X))) ) ) ∨
+        (*4.*) ( (is_atomic A) ∧ (is_release A) ∧ (is_acquire B) ∧ (is_fence B) ∧ (∃ X. (same_address A X) ∧ (sequenced_before g X B) ∧ ((is_read_by g A X) ∨ (∃ Z. (is_read_by g Z X) ∧ (in_release_sequence_of g Z A))  ))  ) ∨ (* TODO *)
         (*5. A is the creation of a thread and B is the beginning of the execution of the new thread. *) (F) ∨
         (*6. A is a futex wake operation and B is the next operation after the futex wait operation of the thread woken up by A. *) (F)   )`;
 
 val (dob_rules, dob_ind, dob_cases) = xHol_reln "dob" `
-      (*1.*) (∀ g A B  . (isRelease A) ∧ (modifiesBefore g A B) ∧ ~(sameThread A B) ∧ (isConsume B) ∧ (∃ X. (inReleaseSequenceOf g X A) ∧ (isReadBy g X B) ) ==> dependencyOrderedBefore g A B  ) ∧
-      (*2.*) (∀ g A B X. (dependencyOrderedBefore g A X) ∧ (carriesDependencyTo g X B) ==> dependencyOrderedBefore g A B)   `;
+      (*1.*) (∀ g A B  . (is_release A) ∧ (modifies_before g A B) ∧ ~(same_thread A B) ∧ (is_consume B) ∧ (∃ X. (in_release_sequence_of g X A) ∧ (is_read_by g X B) ) ==> dependency_ordered_before g A B  ) ∧
+      (*2.*) (∀ g A B X. (dependency_ordered_before g A X) ∧ (carries_dependency_to g X B) ==> dependency_ordered_before g A B)   `;
 
 val (ithb_rules, ithb_ind, ithb_cases) = xHol_reln "ithb" `
-    (* A.  *) ( ∀ g A B  . (synchronizesWith g A B) ==> (interthreadHappensBefore g A B)) ∧
-    (* B.  *) ( ∀ g A B  . (dependencyOrderedBefore g A B) ==> (interthreadHappensBefore g A B)) ∧
-    (* C.1 *) ( ∀ g A B X. ((synchronizesWith g A X) ∧ (sequencedBefore g X B)) ==> (interthreadHappensBefore g A B)) ∧
-    (* C.2 *) ( ∀ g A B X. ((sequencedBefore g A X) ∧ (interthreadHappensBefore g X B)) ==> (interthreadHappensBefore g A B)) ∧
-    (* C.3 *) ( ∀ g A B X. ((interthreadHappensBefore g A X) ∧ (interthreadHappensBefore g X B)) ==> (interthreadHappensBefore g A B)   )`;
+    (* A.  *) ( ∀ g A B  . (synchronizes_with g A B) ==> (interthread_happens_before g A B)) ∧
+    (* B.  *) ( ∀ g A B  . (dependency_ordered_before g A B) ==> (interthread_happens_before g A B)) ∧
+    (* C.1 *) ( ∀ g A B X. ((synchronizes_with g A X) ∧ (sequenced_before g X B)) ==> (interthread_happens_before g A B)) ∧
+    (* C.2 *) ( ∀ g A B X. ((sequenced_before g A X) ∧ (interthread_happens_before g X B)) ==> (interthread_happens_before g A B)) ∧
+    (* C.3 *) ( ∀ g A B X. ((interthread_happens_before g A X) ∧ (interthread_happens_before g X B)) ==> (interthread_happens_before g A B)   )`;
 
-val happensBefore_def = Define`
-    happensBefore g A B = (
-      (*1.*) (sequencedBefore g A B) ∨
-      (*2.*) (interthreadHappensBefore g A B)   )`;
+val happens_before_def = Define`
+    happens_before g A B = (
+      (*1.*) (sequenced_before g A B) ∨
+      (*2.*) (interthread_happens_before g A B)   )`;
 
-val visibleTo_def = Define`
-    visibleTo g A B = ( (isStore A) ∧ (isLoad B) ∧
-      (*1.*) (happensBefore g A B) ∧
-      (*2.*) ~(∃ X. (happensBefore g A X) ∧ (happensBefore g X B))   )`;
+val visible_to_def = Define`
+    visible_to g A B = ( (is_store A) ∧ (is_load B) ∧
+      (*1.*) (happens_before g A B) ∧
+      (*2.*) ~(∃ X. (happens_before g A X) ∧ (happens_before g X B))   )`;
 
 (* TODO: fix to only look at writes and only return a set given a read *)
-val inVisibleSequenceOf_def = Define` (* TODO: fix to only look at writes and only return a set given a read? *)
-    inVisibleSequenceOf g A B =
-      let visible_sequence X = { nd | (nd.address = X.address) ∧ (isStore nd) ∧ (isAtomic nd) ∧
-                                      (      (visibleTo g nd X) ∨ (* The first in sequence *)
-                                             (    ~(happensBefore g X nd) ∧
-                                                   (∃fs. (visibleTo g fs X) ∧
-                                                        (modifiesBefore g fs nd))))} (* the rest *)
+val in_visible_sequence_of_def = Define` (* TODO: fix to only look at writes and only return a set given a read? *)
+    in_visible_sequence_of g A B =
+      let visible_sequence X = { nd | (nd.address = X.address) ∧ (is_store nd) ∧ (is_atomic nd) ∧
+                                      (      (visible_to g nd X) ∨ (* The first in sequence *)
+                                             (    ~(happens_before g X nd) ∧
+                                                   (∃fs. (visible_to g fs X) ∧
+                                                         (modifies_before g fs nd))))} (* the rest *)
       in A IN (visible_sequence B)    `;
 
-val sequentiallyConsistent_def = Define`
-    sequentiallyConsistent g A B = (isSeqCst A ∧ isSeqCst B ∧ orderedBefore g A B)`;
+val sequentially_consistent_def = Define`
+    sequentially_consistent g A B = (is_seq_cst A ∧ is_seq_cst B ∧ ordered_before g A B)`;
 
-val seqCstException_def = Define`
-    seqCstException g X B =
-      let isMostRecentSeqCst n = ( (isInGraph g n) ∧
-                                   (sequentiallyConsistent g n B) ∧ (sameAddress n B) ∧ ~(∃ Y.
-                                   (sequentiallyConsistent g Y B) ∧ (sameAddress Y B) ∧ (sequentiallyConsistent g n Y)))
+val seq_cst_exception_def = Define`
+    seq_cst_exception g X B =
+      let is_most_recent_seq_cst n = ( (is_in_graph g n) ∧
+                                       (sequentially_consistent g n B) ∧ (same_address n B) ∧ ~(∃ Y.
+                                       (sequentially_consistent g Y B) ∧ (same_address Y B) ∧ (sequentially_consistent g n Y)))
       in
-         ( ∃ A. (isMostRecentSeqCst A ∧ ( (X = A) ∨ ( (inVisibleSequenceOf g X B) ∧ ~(isSeqCst X) ∧ ~(happensBefore g X A)))) ∨
-          ~∃ A. (isMostRecentSeqCst A ∧ (inVisibleSequenceOf g X B) ∧ ~(isSeqCst X)))`;
+         ( ∃ A. (is_most_recent_seq_cst A ∧ ( (X = A) ∨ ( (in_visible_sequence_of g X B) ∧ ~(is_seq_cst X) ∧ ~(happens_before g X A)))) ∨
+          ~∃ A. (is_most_recent_seq_cst A ∧ (in_visible_sequence_of g X B) ∧ ~(is_seq_cst X)))`;
 
 
-val canBeReadBy_def = Define`
-    canBeReadBy g B A = (
-      (~(isAtomic A) ∧ ~(isAtomic B) ∧ (visibleTo g B A) ) ∨           (* non-atomic *)
-      (~(isSeqCst B) ∧ (isAtomic A) ∧  (isAtomic B) ∧ (inVisibleSequenceOf g B A) ) ∨ (* atomic *)
-      ( (isSeqCst B) ∧ (sequentiallyConsistent g B A)) ∨                    (* Sequentally Consistent *)
-      ( F )                                                                       (* undefined combinations? *)  )`;
+val can_be_read_by_def = Define`
+    can_be_read_by g B A = (
+      (~(is_atomic A) ∧ ~(is_atomic B) ∧ (visible_to g B A) ) ∨                              (* non-atomic *)
+      (~(is_seq_cst B) ∧ (is_atomic A) ∧  (is_atomic B) ∧ (in_visible_sequence_of g B A) ) ∨ (* atomic *)
+      ( (is_seq_cst B) ∧ (sequentially_consistent g B A)) ∨                                  (* Sequentally Consistent *)
+      ( F )                                                                                  (* undefined combinations? *)  )`;
 
 
 
@@ -181,31 +182,34 @@ val canBeReadBy_def = Define`
 
 (* Receive input message, create new nodes from these messages *)
 val receive_def = Define`
-    receive (inGraph, (msg, ttid)) graph' = case msg of
-      Read a' id order' dep => let new_node = <| operation := Rd ;
-                                             address := a' ;
-                                             values := NONE ;
-                                             mid := id ;
-                                             thread_id := ttid ;
-                                             order := order' ;
-                                             ddeps := dep |>
-                           in (graph' = inGraph with nodes updated_by (λlst. lst ++ [new_node] ))
+  receive (in_graph, (msg, ttid)) graph' =
+    case msg of
+    | Read a' id order' dep =>
+        let new_node = <| operation := Rd;
+                          address := a';
+                          values := NONE;
+                          mid := id;
+                          thread_id := ttid;
+                          order := order';
+                          ddeps := dep |>
+        in (graph' = in_graph with nodes updated_by (λlst. lst ++ [new_node] ))
 
-    | Write a' id vl order' dep => let new_node = <| operation := Wr ;
-                                              address := a' ;
-                                              values := SOME vl ;
-                                              (* mid := LEAST n. ~(∃ nd. (nd.mid = n) ∧ (nd IN inGraph.nodes) ) ;*)
-                                              mid := id;
-                                              thread_id := ttid ;
-                                              order := order' ;
-                                              ddeps := dep |>
-                           in (graph' = inGraph with nodes updated_by (λlst. lst ++ [new_node]))
+    | Write a' id vl order' dep =>
+        let new_node = <| operation := Wr;
+                          address := a';
+                          values := SOME vl;
+                          (* mid := LEAST n. ~(∃ nd. (nd.mid = n) ∧ (nd IN in_graph.nodes));*)
+                          mid := id;
+                          thread_id := ttid;
+                          order := order';
+                          ddeps := dep |>
+        in (graph' = in_graph with nodes updated_by (λlst. lst ++ [new_node]))
 `;
 
 (* TODO: output message *)
 val resolve_def = Define`
     resolve g1 (msg, g2) = ∃ w r. (g1.nodes = g2.nodes) ∧ (* TODO: maybe update r's value? *)
-                                  (canBeReadBy g1 w r) ∧ (g2.rf = g1.rf |+ (r, w)) ∧
+                                  (can_be_read_by g1 w r) ∧ (g2.rf = g1.rf |+ (r, w)) ∧
                                   (~∃ w'. FLOOKUP g1.rf r = SOME w') ∧
                                   (msg = Out (THE w.values) (r.mid) (r.thread_id))
 `;
@@ -216,51 +220,51 @@ val resolve_def = Define`
 (***********************************)
 (* Defined and Undefined Behaviour *)
 (***********************************)
-val dataRace_def = Define`
-    dataRace g A B = (
-       (isInGraph g A)               ∧
-       (isInGraph g B)               ∧
-       (sameAddress A B)             ∧
-       ( (isStore A) ∨ (isStore B) ) ∧
-      ~(happensBefore g A B)         ∧
-      ~(happensBefore g B A)
+val data_race_def = Define`
+    data_race g A B = (
+       (is_in_graph g A)               ∧
+       (is_in_graph g B)               ∧
+       (same_address A B)              ∧
+       ( (is_store A) ∨ (is_store B) ) ∧
+      ~(happens_before g A B)          ∧
+      ~(happens_before g B A)
  )`;
 
 val indeterminate_read_def = Define`
-    indeterminate_read g A = ~∃ B. canBeReadBy g B A`;
+    indeterminate_read g A = ~∃ B. can_be_read_by g B A`;
 
 val consistent_sc_order_def = Define`
     consistent_sc_order g = ∀ A B.
-        (isSeqCst A ∧ isSeqCst B) ==> ((happensBefore g A B ==> sequentiallyConsistent g A B) ∧
-                                       (modifiesBefore g A B ==> sequentiallyConsistent g A B))`;
+        (is_seq_cst A ∧ is_seq_cst B) ==> ((happens_before g A B ==> sequentially_consistent g A B) ∧
+                                          (modifies_before g A B ==> sequentially_consistent g A B))`;
 
 val consistent_reads_from_mapping_def = Define`
-    consistent_reads_from_mapping g = ∀ A B. isReadBy g A B ==> (canBeReadBy g A B ∧ isInGraph g A ∧ isInGraph g B)`;
+    consistent_reads_from_mapping g = ∀ A B. is_read_by g A B ==> (can_be_read_by g A B ∧ is_in_graph g A ∧ is_in_graph g B)`;
 
 val consistent_ithb_def = Define`
-    consistent_ithb g = ∀ A. ~interthreadHappensBefore g A A`;
+    consistent_ithb g = ∀ A. ~interthread_happens_before g A A`;
 
 val consistent_modification_order_def = Define`
     consistent_modification_order g = ∀ A B.
-        ( (isAtomic A ∧ isAtomic B) ==> (happensBefore g A B ==> modifiesBefore g A B)) ∧
-        (~(isAtomic A ∧ isAtomic B) ==> ~modifiesBefore g A B)`;
+        ( (is_atomic A ∧ is_atomic B) ==> (happens_before g A B ==> modifies_before g A B)) ∧
+        (~(is_atomic A ∧ is_atomic B) ==> ~modifies_before g A B)`;
 
 (* Coherence *)
 val CoRR_def = Define`
-    CoRR g = ~∃ A B C D. (happensBefore g C D ∧ isReadBy g A C ∧ isReadBy g B D ∧ modifiesBefore g B A)`;
+    CoRR g = ~∃ A B C D. (happens_before g C D ∧ is_read_by g A C ∧ is_read_by g B D ∧ modifies_before g B A)`;
 
 val CoWR_def = Define`
-    CoWR g = ~∃ B C D. (isReadBy g B D ∧ happensBefore g C D ∧ modifiesBefore g B C)`;
+    CoWR g = ~∃ B C D. (is_read_by g B D ∧ happens_before g C D ∧ modifies_before g B C)`;
 
 val CoWW_def = Define`
-    CoWW g = ~∃ A B. happensBefore g A B ∧ modifiesBefore g B A`;
+    CoWW g = ~∃ A B. happens_before g A B ∧ modifies_before g B A`;
 
 val CoRW_def = Define`
-    CoRW g = let rhm = ($RUNION ( $RUNION (isReadBy g) (happensBefore g)) (modifiesBefore g))
+    CoRW g = let rhm = ($RUNION ( $RUNION (is_read_by g) (happens_before g)) (modifies_before g))
               in (~∃ A. rhm^* A A)`;          
 
-val wellFormed_def = Define`
-    wellFormed g = consistent_reads_from_mapping g`;
+val well_formed_def = Define`
+    well_formed g = consistent_reads_from_mapping g`;
 
 val consistent_execution_def = Define`
     consistent g = (
@@ -269,7 +273,7 @@ val consistent_execution_def = Define`
         consistent_modification_order g ∧
         consistent_reads_from_mapping g ∧
         (* No dataraces *)
-        (~∃ A B. dataRace g A B) ∧
+        (~∃ A B. data_race g A B) ∧
         (* No indeterminate reads *)
         (~∃ A. indeterminate_read g A)
 )`;
@@ -281,143 +285,143 @@ val consistent_execution_def = Define`
 (* Proofs for some properties of the relations defined above *)
 (*************************************************************)
 
-val impliesOB_def = Define`
-    impliesOrderedBefore p = ∀ g A B. (wellFormed g ∧ p g A B ==> orderedBefore g A B)`;
+val implies_ob_def = Define`
+    implies_ordered_before p = ∀ g A B. (well_formed g ∧ p g A B ==> ordered_before g A B)`;
 val trans_def = Define`
     transitive p = ∀ A B C. p A B ∧ p B C ==> p A C`;
 val asym_def = Define`
     assymetric p = ∀ A B. p A B ==> ~p B A`;
 val irrefl_def = Define`
     irreflexive p = ∀ A. ~p A A`;
-val impliesInGraph_def = Define`
-    impliesInGraph p = ∀ g A B. (wellFormed g ∧ p g A B) ==> (isInGraph g A ∧ isInGraph g B)`;
+val implies_in_graph_def = Define`
+    implies_in_graph p = ∀ g A B. (well_formed g ∧ p g A B) ==> (is_in_graph g A ∧ is_in_graph g B)`;
 
 
 
-(* orderedBefore *)
-val orderedBefore_irreflexivity = prove(
-    ``∀ g. irreflexive (orderedBefore g)``,
-        rw [irrefl_def, orderedBefore_def]);
-val orderedBefore_asymmetry = prove(
-    ``∀ g. assymetric (orderedBefore g)``,
-        RW_TAC arith_ss [asym_def,orderedBefore_def]);
-val orderedBefore_transitivity = prove(
-    ``∀g. transitive (orderedBefore g)``,
-        RW_TAC arith_ss [trans_def,orderedBefore_def]);
-(* If something implies orderedBefore then it is also irreflexive and assymetrical *)
-val orderedBefore_inGraph = prove(
-    ``impliesInGraph orderedBefore``, rw [impliesInGraph_def, orderedBefore_def]);
+(* ordered_before *)
+val ordered_before_irreflexivity = prove(
+    ``∀ g. irreflexive (ordered_before g)``,
+        rw [irrefl_def, ordered_before_def]);
+val ordered_before_asymmetry = prove(
+    ``∀ g. assymetric (ordered_before g)``,
+        RW_TAC arith_ss [asym_def,ordered_before_def]);
+val ordered_before_transitivity = prove(
+    ``∀g. transitive (ordered_before g)``,
+        RW_TAC arith_ss [trans_def,ordered_before_def]);
+(* If something implies ordered_before then it is also irreflexive and assymetrical *)
+val ordered_before_in_graph = prove(
+    ``implies_in_graph ordered_before``, rw [implies_in_graph_def, ordered_before_def]);
 
-val isReadBy_inGraph = prove(
-    ``impliesInGraph isReadBy``, prove_tac [impliesInGraph_def, consistent_reads_from_mapping_def,wellFormed_def]);
+val is_read_by_in_graph = prove(
+    ``implies_in_graph is_read_by``, prove_tac [implies_in_graph_def, consistent_reads_from_mapping_def,well_formed_def]);
 
-(* modifiesBefore *)
-val modifiesBefore_orderedBefore = prove(
-    ``∀ g A B. modifiesBefore g A B ==> orderedBefore g A B``,
-        RW_TAC (srw_ss()) [modifiesBefore_def]);
-val modifiesBefore_transitivity = prove(
-    ``∀ g. transitive (modifiesBefore g)``,
-        METIS_TAC [trans_def, modifiesBefore_def,sameAddress_def, orderedBefore_transitivity]);
-val modifiesBefore_inGraph = prove(
-    ``impliesInGraph modifiesBefore``, metis_tac[impliesInGraph_def,orderedBefore_inGraph,modifiesBefore_def]);
+(* modifies_before *)
+val modifies_before_ordered_before = prove(
+    ``∀ g A B. modifies_before g A B ==> ordered_before g A B``,
+        RW_TAC (srw_ss()) [modifies_before_def]);
+val modifies_before_transitivity = prove(
+    ``∀ g. transitive (modifies_before g)``,
+        METIS_TAC [trans_def, modifies_before_def,same_address_def, ordered_before_transitivity]);
+val modifies_before_in_graph = prove(
+    ``implies_in_graph modifies_before``, metis_tac[implies_in_graph_def,ordered_before_in_graph,modifies_before_def]);
 
-(* sequencedBefore *)
-val sequencedBefore_orderedBefore = prove(
-    ``∀ g A B. sequencedBefore g A B ==> orderedBefore g A B``,
-        RW_TAC (srw_ss()) [sequencedBefore_def]);
-val sequencedBefore_transitivity = prove(
-    ``∀ g. transitive (sequencedBefore g)``,
-        METIS_TAC [trans_def, sequencedBefore_def,orderedBefore_transitivity,sameThread_def]);
-val sequencedBefore_inGraph = prove(
-    ``impliesInGraph sequencedBefore``, metis_tac[impliesInGraph_def,orderedBefore_inGraph,sequencedBefore_def]);
+(* sequenced_before *)
+val sequenced_before_ordered_before = prove(
+    ``∀ g A B. sequenced_before g A B ==> ordered_before g A B``,
+        RW_TAC (srw_ss()) [sequenced_before_def]);
+val sequenced_before_transitivity = prove(
+    ``∀ g. transitive (sequenced_before g)``,
+        METIS_TAC [trans_def, sequenced_before_def,ordered_before_transitivity,same_thread_def]);
+val sequenced_before_in_graph = prove(
+    ``implies_in_graph sequenced_before``, metis_tac[implies_in_graph_def,ordered_before_in_graph,sequenced_before_def]);
 
-(* releaseSequenceOf *)
-val inReleaseSequenceOf_selfOrderedBefore = prove(
-    ``∀ g A B. inReleaseSequenceOf g A B ∧ (A <> B) ==> orderedBefore g B A``,
-        RW_TAC(srw_ss()) [inReleaseSequenceOf_def,sequencedBefore_def]);
-(*val inReleaseSequenceOf_headOrderedBefore = prove(
-    ``∀ g A B C. isReadBy g B C ∧ inReleaseSequenceOf g B A ==> orderedBefore g A C``,
-        METIS_TAC [trans_def, isReadBy_def,inReleaseSequenceOf_selfOrderedBefore,orderedBefore_transitivity]);*)
-val inReleaseSequenceOf_reflexivity = prove(
-    ``∀ g A. isInGraph g A ==> inReleaseSequenceOf g A A``,
-        rw [inReleaseSequenceOf_def]);
-val inReleaseSequenceOf_transitivity = prove(
-    ``∀ g A B C. inReleaseSequenceOf g A B ∧ inReleaseSequenceOf g B C ==> inReleaseSequenceOf g A C``,
-        RW_TAC arith_ss [trans_def,inReleaseSequenceOf_def, orderedBefore_transitivity] THEN
-        METIS_TAC [trans_def,sequencedBefore_transitivity,modifiesBefore_transitivity]);
-val inReleaseSequenceOf_inGraph = prove(
-    ``impliesInGraph inReleaseSequenceOf``,
-        rw [impliesInGraph_def,inReleaseSequenceOf_def,sequencedBefore_def,orderedBefore_def] >> rw []);
+(* release_sequence_of *)
+val in_release_sequence_of_self_ordered_before = prove(
+    ``∀ g A B. in_release_sequence_of g A B ∧ (A <> B) ==> ordered_before g B A``,
+        RW_TAC(srw_ss()) [in_release_sequence_of_def,sequenced_before_def]);
+(*val in_release_sequence_of_headOrderedBefore = prove(
+    ``∀ g A B C. is_read_by g B C ∧ in_release_sequence_of g B A ==> ordered_before g A C``,
+        METIS_TAC [trans_def, is_read_by_def,in_release_sequence_of_self_ordered_before,ordered_before_transitivity]);*)
+val in_release_sequence_of_reflexivity = prove(
+    ``∀ g A. is_in_graph g A ==> in_release_sequence_of g A A``,
+        rw [in_release_sequence_of_def]);
+val in_release_sequence_of_transitivity = prove(
+    ``∀ g A B C. in_release_sequence_of g A B ∧ in_release_sequence_of g B C ==> in_release_sequence_of g A C``,
+        RW_TAC arith_ss [trans_def,in_release_sequence_of_def, ordered_before_transitivity] THEN
+        METIS_TAC [trans_def,sequenced_before_transitivity,modifies_before_transitivity]);
+val in_release_sequence_of_in_graph = prove(
+    ``implies_in_graph in_release_sequence_of``,
+        rw [implies_in_graph_def,in_release_sequence_of_def,sequenced_before_def,ordered_before_def] >> rw []);
 
-(* carriesDependencyTo *)
-val carriesDependencyTo_inGraph = prove(
-    ``impliesInGraph carriesDependencyTo``,
-        rw [impliesInGraph_def,carriesDependencyTo_def]);    
+(* carries_dependency_to *)
+val carries_dependency_to_in_graph = prove(
+    ``implies_in_graph carries_dependency_to``,
+        rw [implies_in_graph_def,carries_dependency_to_def]);    
 
-(* synchronizesWith *)
-val synchronizesWith_inGraph = prove(
-    ``impliesInGraph synchronizesWith``,
-        rw [impliesInGraph_def, synchronizesWith_def] THEN metis_tac [inReleaseSequenceOf_inGraph,impliesInGraph_def,isReadBy_inGraph,sequencedBefore_inGraph]);
+(* synchronizes_with *)
+val synchronizes_with_in_graph = prove(
+    ``implies_in_graph synchronizes_with``,
+        rw [implies_in_graph_def, synchronizes_with_def] THEN metis_tac [in_release_sequence_of_in_graph,implies_in_graph_def,is_read_by_in_graph,sequenced_before_in_graph]);
 
-(* dependencyOrderedBefore *)
-val dob_inGraph = prove(
-    ``impliesInGraph dependencyOrderedBefore``,
-        rw [impliesInGraph_def] >>
-        UNDISCH_TAC ``wellFormed g`` >>
-        UNDISCH_TAC ``dependencyOrderedBefore g A B`` >>
+(* dependency_ordered_before *)
+val dob_in_graph = prove(
+    ``implies_in_graph dependency_ordered_before``,
+        rw [implies_in_graph_def] >>
+        UNDISCH_TAC ``well_formed g`` >>
+        UNDISCH_TAC ``dependency_ordered_before g A B`` >>
         SPEC_TAC (``B:node``,``B:node``) >>
         SPEC_TAC (``A:node``,``A:node``) >>
         SPEC_TAC (``g:graph``,``g:graph``) >>
-        Induct_on `dependencyOrderedBefore` >>
-        rw [] >> metis_tac [impliesInGraph_def, modifiesBefore_inGraph,carriesDependencyTo_def]);
+        Induct_on `dependency_ordered_before` >>
+        rw [] >> metis_tac [implies_in_graph_def, modifies_before_in_graph,carries_dependency_to_def]);
 
-(* interthreadHappensBefore *)
-val ithb_inGraph = prove(
-    ``impliesInGraph interthreadHappensBefore``,
-        rw [impliesInGraph_def] >>
-        UNDISCH_TAC ``wellFormed g`` >>
-        UNDISCH_TAC ``interthreadHappensBefore g A B`` >>
+(* interthread_happens_before *)
+val ithb_in_graph = prove(
+    ``implies_in_graph interthread_happens_before``,
+        rw [implies_in_graph_def] >>
+        UNDISCH_TAC ``well_formed g`` >>
+        UNDISCH_TAC ``interthread_happens_before g A B`` >>
         SPEC_TAC (``B:node``,``B:node``) >>
         SPEC_TAC (``A:node``,``A:node``) >>
         SPEC_TAC (``g:graph``,``g:graph``) >>
-        Induct_on `interthreadHappensBefore` >>
+        Induct_on `interthread_happens_before` >>
         rw [] >>
-        metis_tac [impliesInGraph_def,synchronizesWith_inGraph, dob_inGraph,sequencedBefore_inGraph,synchronizesWith_inGraph]);
+        metis_tac [implies_in_graph_def,synchronizes_with_in_graph, dob_in_graph,sequenced_before_in_graph,synchronizes_with_in_graph]);
 
-(* happensBefore *)
-val happensBefore_partial_transitivity = prove(
-    ``∀ g. (~∃ X. (isInGraph g X ∧ isConsume X)) ==> transitive (happensBefore g)``,
+(* happens_before *)
+val happens_before_partial_transitivity = prove(
+    ``∀ g. (~∃ X. (is_in_graph g X ∧ is_consume X)) ==> transitive (happens_before g)``,
     cheat); (*TODO*)
     
-(* visibleTo *)
-(*val visibleTo_orderedBefore = prove(
-    ``impliesOrderedBefore visibleTo``,
-        METIS_TAC [impliesOB_def, visibleTo_def, happensBefore_orderedBefore]);*)
-(* visibleTo is not transitive, since happensBefore isn't transitive *)
+(* visible_to *)
+(*val visible_to_ordered_before = prove(
+    ``implies_ordered_before visible_to``,
+        METIS_TAC [implies_ob_def, visible_to_def, happens_before_ordered_before]);*)
+(* visible_to is not transitive, since happens_before isn't transitive *)
 
 
-(* inVisibleSequenceOf *)
-(*val inVisibleSequenceOf_irreflexivity = prove(
-    ``∀ g. wellFormed g ==> irreflexive (inVisibleSequenceOf g)``,
-        RW_TAC (srw_ss()) [irrefl_def, LET_THM, inVisibleSequenceOf_def, visibleTo_def] >>
-        `~visibleTo g A A ∧ ~happensBefore g A A` by METIS_TAC [wellFormed_def, irrefl_def, impliesOB_def,visibleTo_orderedBefore, happensBefore_orderedBefore, orderedBefore_irreflexivity] >>
-        Cases_on `isStore A` >> Cases_on `isAtomic A` >> rw [] >>
-        `~isLoad A` by EVAL_TAC >> UNDISCH_TAC ``isStore A`` >> rw [isStore_def,isLoad_def]);*)
-(* inVisibleSequenceOf DOESN'T imply orderedBefore (see example in tests/) *)
+(* in_visible_sequence_of *)
+(*val in_visible_sequence_of_irreflexivity = prove(
+    ``∀ g. well_formed g ==> irreflexive (in_visible_sequence_of g)``,
+        RW_TAC (srw_ss()) [irrefl_def, LET_THM, in_visible_sequence_of_def, visible_to_def] >>
+        `~visible_to g A A ∧ ~happens_before g A A` by METIS_TAC [well_formed_def, irrefl_def, implies_ob_def,visible_to_ordered_before, happens_before_ordered_before, ordered_before_irreflexivity] >>
+        Cases_on `is_store A` >> Cases_on `is_atomic A` >> rw [] >>
+        `~is_load A` by EVAL_TAC >> UNDISCH_TAC ``is_store A`` >> rw [is_store_def,is_load_def]);*)
+(* in_visible_sequence_of DOESN'T imply ordered_before (see example in tests/) *)
 
 
-(* sequentiallyConsistent *)
-(*val sequentiallyConsistent_irreflexivity = prove(
-    ``∀ g. wellFormed g ==> irreflexive (sequentiallyConsistent g)``,
-        METIS_TAC [wellFormed_def, irrefl_def, LET_THM, sequentiallyConsistent_def, inVisibleSequenceOf_irreflexivity, sameAddress_def, orderedBefore_irreflexivity]);*)
-(* sequentiallyConsistent doesn't imply orderedBefore (see inVisibleSequenceOf) *)
+(* sequentially_consistent *)
+(*val sequentially_consistent_irreflexivity = prove(
+    ``∀ g. well_formed g ==> irreflexive (sequentially_consistent g)``,
+        METIS_TAC [well_formed_def, irrefl_def, LET_THM, sequentially_consistent_def, in_visible_sequence_of_irreflexivity, same_address_def, ordered_before_irreflexivity]);*)
+(* sequentially_consistent doesn't imply ordered_before (see in_visible_sequence_of) *)
 
 
-(* canBeReadBy *)
-(*val canBeReadBy_irreflexivity = prove(
-    ``∀ g. wellFormed g ==> irreflexive (canBeReadBy g)``,
-        METIS_TAC [wellFormed_def, irrefl_def,impliesOB_def, canBeReadBy_def, sequentiallyConsistent_irreflexivity,inVisibleSequenceOf_irreflexivity,visibleTo_orderedBefore,orderedBefore_irreflexivity]);*)
-(* canBeReadBy doesn't imply orderedBefore (see seqConsistent) *)
+(* can_be_read_by *)
+(*val can_be_read_by_irreflexivity = prove(
+    ``∀ g. well_formed g ==> irreflexive (can_be_read_by g)``,
+        METIS_TAC [well_formed_def, irrefl_def,implies_ob_def, can_be_read_by_def, sequentially_consistent_irreflexivity,in_visible_sequence_of_irreflexivity,visible_to_ordered_before,ordered_before_irreflexivity]);*)
+(* can_be_read_by doesn't imply ordered_before (see seq_consistent) *)
 
 
 
@@ -428,25 +432,25 @@ val happensBefore_partial_transitivity = prove(
 
 (*open finite_mapTheory;*)
 (*
-val resolve_visibleTo = prove(
-    ``∀ g1 g2 msg A B. resolve g1 (msg, g2) ∧ visibleTo g1 A B ==> visibleTo g2 A B``,
-        rw [resolve_def, visibleTo_def]
+val resolve_visible_to = prove(
+    ``∀ g1 g2 msg A B. resolve g1 (msg, g2) ∧ visible_to g1 A B ==> visible_to g2 A B``,
+        rw [resolve_def, visible_to_def]
 
     
-val resolve_canBeReadBy = prove(
-    ``∀ g1 g2 msg A B. resolve g1 (msg, g2) ∧ canBeReadBy g1 A B ==> canBeReadBy g2 A B``,
-        rw [resolve_def,canBeReadBy_def] THENL [
-          (*1.*)  FULL_SIMP_TAC (srw_ss()) [inVisibleSequenceOf_def,sequentiallyConsistent_def,visibleTo_def,LET_THM,visibleTo_def,orderedBefore_def,happensBefore_def]
+val resolve_can_be_read_by = prove(
+    ``∀ g1 g2 msg A B. resolve g1 (msg, g2) ∧ can_be_read_by g1 A B ==> can_be_read_by g2 A B``,
+        rw [resolve_def,can_be_read_by_def] THENL [
+          (*1.*)  FULL_SIMP_TAC (srw_ss()) [in_visible_sequence_of_def,sequentially_consistent_def,visible_to_def,LET_THM,visible_to_def,ordered_before_def,happens_before_def]
         ]
            METIS_TAC []
            
-val resolve_wellFormed = prove(
-    ``∀ g1 g2 msg. wellFormed g1 ∧ resolve g1 (msg, g2) ==> wellFormed g2``,
-        rw [wellFormed_def] THENL [
-            metis_tac [resolve_def,orderedBefore_def,carriesDependencyTo_def],
+val resolve_well_formed = prove(
+    ``∀ g1 g2 msg. well_formed g1 ∧ resolve g1 (msg, g2) ==> well_formed g2``,
+        rw [well_formed_def] THENL [
+            metis_tac [resolve_def,ordered_before_def,carries_dependency_to_def],
             FULL_SIMP_TAC (srw_ss()) [resolve_def]>>
             Cases_on `(r,w)=(B,A)` >> rw [] >>
-            FULL_SIMP_TAC (srw_ss()) [isReadBy_def]
+            FULL_SIMP_TAC (srw_ss()) [is_read_by_def]
             Cases_on `r=B` >> rw []
             `(g1.rf |+ (B,w)) ' B = A ∧ w = A` by FULL_SIMP_TAC (srw_ss()) [FLOOKUP_DEF] THENL [
                 METIS_TAC [FLOOKUP_DEF,FAPPLY_FUPDATE_THM],
@@ -460,8 +464,8 @@ val resolve_wellFormed = prove(
 
 (* TODO:
 
-1. Find example where A isReadBy B but B is orderedBefore A
-2. Find example where A is orderedBefore B but B is in the visibleSequence of A
+1. Find example where A is_read_by B but B is ordered_before A
+2. Find example where A is ordered_before B but B is in the visible_sequence of A
 
  *)
 
