uvmSystemScript.sml
@@ -9,9 +9,12 @@ open uvmIRTheory;
 val _ = new_theory "uvmSystem"; 
 
 
-val machineState_def = Datatype`
-    machineState = <| g : graph ;
-                      tsList : threadState list |>`;
+val machine_state_def = Datatype`
+   machine_state = <|
+     g : graph;
+     ts_list : thread_state list
+   |>
+`;
 
 val _ = Datatype`
   msstep_result = SuccessM α | AbortM | BlockedM
@@ -20,7 +23,7 @@ val _ = Datatype`
 (* set up MSM, a monad *)
 val _ = type_abbrev(
   "MSM",
-  ``:machineState -> (α # machineState) msstep_result``)
+  ``:machine_state -> (α # machine_state) msstep_result``)
 
 val MSUNIT_def = Define`
   MSUNIT (x:α) :α MSM = λms. SuccessM (x, ms)
@@ -32,10 +35,10 @@ val MSBIND_def = Define`
   MSBIND (x : α MSM) (f : α -> β MSM) : β MSM =
     λms0.
       case x ms0 of
-      | SuccessM (a, ms1) =>
-        (case f a ms1 of
-         | SuccessM(b, ms2) => SuccessM(b, ms2)
-         | r => r)
+      | SuccessM (a, ms1) => (
+          case f a ms1 of
+          | SuccessM(b, ms2) => SuccessM(b, ms2)
+          | r => r)
       | AbortM => AbortM
       | BlockedM => BlockedM
 `;
@@ -45,113 +48,136 @@ val _ = overload_on ("monad_unitbind", ``λm1 m2. MSBIND m1 (K m2)``)
 
 
 val MSGET_def = Define`
-  MSGET : machineState MSM = λms. SuccessM(ms, ms)
+  MSGET : machine_state MSM = λms. SuccessM(ms, ms)
 `
 
-val readVar_def = Define`
-readVar (x : num) : (graph) MSM =
-        do
-            ms <- MSGET ;
-            return ms.g
-        od
+val read_var_def = Define`
+  read_var (x : num) : (graph) MSM =
+    do
+      ms <- MSGET ;
+      return ms.g
+    od
 `;
 
 val eval_exp_def = Define`
   eval_exp (e:num) : (value # value) MSM =
-      return ((Int 32 1), (Int 32 8))
+    return ((Int 32 1), (Int 32 8))
 `
 
 val valbind_def = Define`
   valbind : unit MSM =
     do
-             λms. SuccessM((), ms)
+      λms. SuccessM((), ms)
     od
 `;
 
-val findNodeFun_def = Define`
-findNodeFun list (n,tid) = case list of
-                               [] => NONE
-                             | x::xs => if (x.mid = n ∧ x.thread_id = tid) then SOME x else findNodeFun xs (n,tid)`;
-val findNode_def = Define`
-findNode (n,tid) : (node option) MSM =
-                               do
-                                   ms <- MSGET ;
-                                   return (findNodeFun (ms.g.nodes) (n,tid))
-                               od
+val find_node_fun_def = Define`
+  find_node_fun list (n,tid) =
+    case list of
+    | [] => NONE
+    | x::xs => if (x.mid = n ∧ x.thread_id = tid) then SOME x else find_node_fun xs (n,tid)
+`;
+
+val find_node_def = Define`
+  find_node (n,tid) : (node option) MSM =
+    do
+      ms <- MSGET ;
+      return (find_node_fun (ms.g.nodes) (n,tid))
+    od
 `;
 
 val resolveM_def = Define`
-    resolveM R W : memoryMessageResolve MSM =
-      λms. SuccessM(ResolvedRead (THE W.values) R.mid, ms with g updated_by (λgr. gr with rf updated_by (λr. r|+(R,W) )   )    )`;
+  resolveM R W : memory_message_resolve MSM =
+    λms. SuccessM(ResolvedRead (THE W.values) R.mid, ms with g updated_by (λgr. gr with rf updated_by (λr. r|+(R,W))))
+`;
 
-val listUpdate_def = Define`
-    listUpdate list index v = case list of
-        [] => []
-      | x::xs => if(index=0)then(v::xs)else(x::(listUpdate xs (index-1) v))`;
+val list_update_def = Define`
+  list_update list index v =
+    case list of
+    | [] => []
+    | x::xs => if (index=0) then (v::xs) else (x::(list_update xs (index-1) v))
+`;
 
-val threadReceiveM_def = Define`
-    threadReceiveM msg tid : unit MSM =
-      λms. SuccessM (  (),  <| g:= ms.g ; tsList := listUpdate ms.tsList tid (threadReceive (EL tid ms.tsList) msg) |>)
+val thread_receiveM_def = Define`
+  thread_receiveM msg tid : unit MSM =
+    λms. SuccessM ((),  <| g := ms.g ; ts_list := list_update ms.ts_list tid (thread_receive (EL tid ms.ts_list) msg) |>)
 `;
 
 
-val getResult_def = Define`
-    getResult (r:(unit # threadState # memoryMessage list) tsstep_result) : (unit # threadState # memoryMessage list) MSM = case r of
-      | Success α => return α`;
+val get_result_def = Define`
+  get_result (r:(unit # thread_state # memory_message list) tsstep_result) : (unit # thread_state # memory_message list) MSM =
+    case r of
+    | Success α => return α
+`;
 
-val runInst_def = Define`
-    runInst inst t1 : (memoryMessage list) MSM = 
-      do
-          ms0 <- MSGET ;
-          (a,ts1,msg) <- getResult (exec_inst inst (EL t1 ms0.tsList)) ;
-          λms. SuccessM ( msg, <| g:= ms.g ; tsList := listUpdate ms.tsList t1 ts1 |>)
-      od`;
+val run_inst_def = Define`
+  run_inst inst t1 : (memory_message list) MSM = 
+    do
+      ms0 <- MSGET ;
+      (a,ts1,msg) <- get_result (exec_inst inst (EL t1 ms0.ts_list)) ;
+      λms. SuccessM ( msg, <| g:= ms.g ; ts_list := list_update ms.ts_list t1 ts1 |>)
+    od
+`;
 
-type_of(``getResult(exec_inst inst (EL t1 ms.tsList))``);
-type_of(``SuccessM ( msg, <| g:= ms.g ; tsList := listUpdate ms.tsList t1 ts1 |>)``);
+type_of(``get_result(exec_inst inst (EL t1 ms.ts_list))``);
+type_of(``SuccessM ( msg, <| g:= ms.g ; ts_list := list_update ms.ts_list t1 ts1 |>)``);
 
 val receiveH_def = Define`
-    receiveH inGraph (msg,ttid) = case msg of
-        Read a' id order' dep => let new_node = <| operation := Rd ; address := a' ;
-                                     values := NONE      ; mid := id ;
-                                     thread_id := ttid   ; order := order' ;
-                                     ddeps := dep |>
-                                 in inGraph with nodes updated_by (λlst. lst ++ [new_node])
-      | Write a' id vl order' dep => let new_node = <| operation := Wr ;
-                                         address := a'   ; values := SOME vl ;
-                                         mid := id       ; thread_id := ttid ;
-                                         order := order' ; ddeps := dep |>
-                                     in inGraph with nodes updated_by (λlst. lst ++ [new_node])  `;
+  receiveH inGraph (msg,ttid) =
+    case msg of
+    | Read a' id order' dep =>
+        let new_node = <|
+              operation := Rd ;
+              address := a'   ; values := NONE    ;
+              mid := id       ; thread_id := ttid ;
+              order := order' ; ddeps := dep
+            |>
+        in inGraph with nodes updated_by (λlst. lst ++ [new_node])
+    | Write a' id vl order' dep =>
+        let new_node = <|
+              operation := Wr ;
+              address := a'   ; values := SOME vl ;
+              mid := id       ; thread_id := ttid ;
+              order := order' ; ddeps := dep
+            |>
+        in inGraph with nodes updated_by (λlst. lst ++ [new_node])
+`;
 
-val receiveList_def = Define`
-    receiveList g (messages,tid) = case messages of
-      | [] => g
-      | m::rest => receiveList (receiveH g (m,tid)) (rest,tid)`;
+val receive_list_def = Define`
+  receive_list g (messages,tid) =
+    case messages of
+    | [] => g
+    | m::rest => receive_list (receiveH g (m,tid)) (rest,tid)
+`;
 
 val receiveM_def = Define`
-    receiveM messages tid : unit MSM = λms. SuccessM ((), <| g := receiveList ms.g (messages,tid) ; tsList := ms.tsList |>)`;
-
-
-val _ = Datatype` command = read (memreqid # tid) (memreqid # tid)
-                          | eval (instruction # tid)`;
-
-val machine_step_def = Define`
-machine_step com : unit MSM =
-      case com of
-           read (r,t1) (w,t2) =>
-             do
-                 read  <- findNode (r,t1) ;
-                 write <- findNode (w,t2) ;
-                 msg <- resolveM (THE read) (THE write) ;
-                 threadReceiveM msg t1
-             od
-         | eval (inst, t1) =>
-             do
-                 messages <- runInst inst t1;
-                 receiveM messages t1
-             od
+  receiveM messages tid : unit MSM =
+    λms. SuccessM ((), <| g := receive_list ms.g (messages,tid) ; ts_list := ms.ts_list |>)
 `;
 
 
+val _ = Datatype`
+  command =
+  | read (memreqid # tid) (memreqid # tid)
+  | eval (instruction # tid)
+`;
+
+val machine_step_def = Define`
+  machine_step com : unit MSM =
+    case com of
+    | read (r,t1) (w,t2) =>
+        do
+          read  <- find_node (r,t1) ;
+          write <- find_node (w,t2) ;
+          msg <- resolveM (THE read) (THE write) ;
+          thread_receiveM msg t1
+        od
+    | eval (inst, t1) =>
+        do
+          messages <- run_inst inst t1;
+          receiveM messages t1
+        od
+`;
 
 val _ = export_theory();
+
