uvmValuesScript.sml
@@ -14,47 +14,48 @@ val _ = type_abbrev("int",     ``:num``)
 
 
 val _ = Datatype`
-   value =
-     Int num int
-   | IRef uvmType addr
-   | FloatV float32
-   | DoubleV float64
-   (* not sure if these are storable-in-register values
-   | StructV (value list)
-   | ArrayV (value list)
-   | Hybrid (value list) (value list) *)
-   | VectorV (value list)
-   | FuncRefV addr
-   | UFuncRefV addr
+  value =
+  | Int num int
+  | IRef uvm_type addr
+  | FloatV float32
+  | DoubleV float64
+  (* not sure if these are storable-in-register values
+  | StructV (value list)
+  | ArrayV (value list)
+  | Hybrid (value list) (value list) *)
+  | VectorV (value list)
+  | FuncRefV addr
+  | UFuncRefV addr
 `;
 
 (* TEMPORARY *)
 val Int32_def = Define`
-    Int32 = Int 32`;
+  Int32 = Int 32`;
 
 val value_add_def = Define`
-value_add v1 v2 =
-     case (v1, v2) of
-         (Int sz1 n1, Int sz2 n2) => if sz1 = sz2 then SOME (Int sz1 (n1 + n2))
-                                     else NONE
-      |  (Int _ _, _) => NONE
-      | _ => NONE
+  value_add v1 v2 =
+    case (v1, v2) of
+    | (Int sz1 n1, Int sz2 n2) => if sz1 = sz2 then SOME (Int sz1 (n1 + n2))
+                                  else NONE
+    | (Int _ _, _) => NONE
+    | _ => NONE
 `;
 val _ = overload_on ("+", ``value_add``);
 
 val value_div_def = Define`
-    value_div v1 v2 =
-             case (v1,v2) of
-                 (Int sz1 n1, Int sz2 n2) => if (sz2=sz1 ∧ n2<>0) then SOME (Int sz1 (n1 DIV n2))
-                                             else NONE
-               | _ => NONE
+  value_div v1 v2 =
+    case (v1,v2) of
+    | (Int sz1 n1, Int sz2 n2) => if (sz2=sz1 ∧ n2<>0) then SOME (Int sz1 (n1 DIV n2))
+                                  else NONE
+    | _ => NONE
 `;
 val _ = overload_on ("DIV", ``value_div``);
 
 val value_to_address = Define`
-    value_to_address (v:value) : (addr option) = case v of
-        Int sz1 n1 => SOME n1
-      | _ => NONE
+  value_to_address (v:value) : (addr option) =
+    case v of
+    | Int sz1 n1 => SOME n1
+    | _ => NONE
 `;
-                    
+
 val _ = export_theory();
